Moved sim_state to a new file SimState.v. Split Promise.v to PromiseLTS.v and PromiseOutcome.v. Put some lemmas to more appropriate files.

src/promiseToImm/PromiseOutcome.v
@@ -4,31 +4,10 @@ Require Import Prog.
 Require Import ProgToExecution.
 Require Import Events.
 Require Import Event_imm_promise.
+Require Import PromiseLTS.
 
 Set Implicit Arguments.
 Remove Hints plus_n_O.
-
-Definition lts_step (tid : thread_id) (pe : Event.ProgramEvent.t) (s1 s2 : state) : Prop :=
-  exists (labels : list label),
-    ⟪ISTEP: istep tid labels s1 s2⟫ /\
-    ⟪LABS : lab_imm_promise labels pe⟫.
-
-Lemma istep_nil_eq_silent thread :
-  istep thread nil ≡
-  lts_step thread ProgramEvent.silent.
-Proof.
-  unfold lts_step. unfold lab_imm_promise.
-  split.
-  { intros x y H. exists nil. by split. }
-  intros x y H. desf.
-Qed.
-
-Definition thread_lts (tid : thread_id) : Language.t :=
-  @Language.mk
-    (list Instr.t) state
-    init
-    is_terminal
-    (lts_step tid).
 
 Definition init_threads (prog : Prog.t) : Threads.syntax :=
   IdentMap.mapi (fun tid (linstr : list Instr.t) => existT _ (thread_lts tid) linstr) prog.
