src/promiseToImm/PromiseLTS.v
@@ -1,0 +1,21 @@
+From hahn Require Import Hahn.
+From promising Require Import Language.
+Require Import Prog.
+Require Import ProgToExecution.
+Require Import Events.
+Require Import Event_imm_promise.
+
+Set Implicit Arguments.
+Remove Hints plus_n_O.
+
+Definition lts_step (tid : thread_id) (pe : Event.ProgramEvent.t) (s1 s2 : state) : Prop :=
+  exists (labels : list label),
+    ⟪ISTEP: istep tid labels s1 s2⟫ /\
+    ⟪LABS : lab_imm_promise labels pe⟫.
+
+Definition thread_lts (tid : thread_id) : Language.t :=
+  @Language.mk
+    (list Instr.t) state
+    init
+    is_terminal
+    (lts_step tid).
