src/promiseToImm/RMWPlainStep.v
@@ -26,8 +26,9 @@ Require Import SimulationRelAux.
 Require Import PlainStepBasic.
 Require Import ReadPlainStepHelper.
 
+Require Import SimState.
 Require Import SimStateHelper.
-Require Import Promise.
+Require Import PromiseLTS.
 Require Import ProgToExecution.
 Require Import Arith.
 Require Import MemoryAux.
