src/promiseToImm/SimState.v
@@ -1,0 +1,36 @@
+From hahn Require Import Hahn.
+From promising Require Import Language.
+
+Require Import Events Execution.
+Require Import ProgToExecution.
+Require Import ProgToExecutionProperties.
+Require Import PromiseLTS.
+
+Set Implicit Arguments.
+
+Inductive sim_mode := sim_normal | sim_certification.
+  
+Definition sim_state_helper G smode thread
+           (state state' : Language.state (thread_lts thread)) : Prop :=
+  ⟪ STEPS : (step thread)＊ state state' ⟫ /\
+  ⟪ TERMINAL : smode = sim_normal -> is_terminal state' ⟫ /\
+  ⟪ TEH  : thread_restricted_execution G thread state'.(ProgToExecution.G) ⟫.
+
+Definition sim_state G smode (C : actid -> Prop) thread
+           (state : Language.state (thread_lts thread)) : Prop :=
+  ⟪ PCOV : forall index , C (ThreadEvent thread index) <-> index < state.(eindex)⟫ /\
+  exists state', sim_state_helper G smode state state'.
+
+Lemma sim_state_other_thread_step G
+      (C C' : actid -> Prop) smode thread (state : Language.state (thread_lts thread))
+      (CINCL : C ⊆₁ C')
+      (COVSTEP : forall a, tid a = thread -> C' a -> C a)
+      (SIMSTATE: sim_state G smode C state) :
+  sim_state G smode C' state.
+Proof.
+  cdes SIMSTATE.
+  red. splits; eauto.
+  ins. split; ins.
+  { apply PCOV. apply COVSTEP; eauto. }
+  apply CINCL. by apply PCOV.
+Qed.
